I know this will break many things

AwsCryptographicMaterialProviders/dafny/AwsCryptographyKeyStore/src/Structure.dfy
@@ -2,6 +2,7 @@
 // SPDX-License-Identifier: Apache-2.0
 
 include "../Model/AwsCryptographyKeyStoreTypes.dfy"
+include "./PrefixUtils.dfy"
 
 module {:options "/functionSyntax:4" } Structure {
   import opened Wrappers
@@ -10,6 +11,7 @@ module {:options "/functionSyntax:4" } Structure {
   import Types = AwsCryptographyKeyStoreTypes
   import DDB = ComAmazonawsDynamodbTypes
   import UTF8
+  import PrefixUtils
 
   //Attribute Names
   const BRANCH_KEY_IDENTIFIER_FIELD := "branch-key-id"
@@ -78,40 +80,17 @@ module {:options "/functionSyntax:4" } Structure {
               forall
                 reserved <- BRANCH_KEY_RESTRICTED_FIELD_NAMES
                 ::
-                  !( ENCRYPTION_CONTEXT_PREFIX <= reserved) && !(ENCRYPTION_CONTEXT_PREFIX < reserved)
+                  !( ENCRYPTION_CONTEXT_PREFIX <= reserved) //&& !(ENCRYPTION_CONTEXT_PREFIX < reserved)
             )
   {
-    //HierarchyVersionIsNotPrefixed();
-    assert && ENCRYPTION_CONTEXT_PREFIX[0] as char == 'a' as char
-           && HIERARCHY_VERSION[0] == 'h'
-           && "a" != "h";
+    HierarchyVersionIsNotPrefixed();
   }
 
-  lemma RestrictedStringsAreNotPrefixed(s: string)
-    ensures s in BRANCH_KEY_RESTRICTED_FIELD_NAMES ==> !(ENCRYPTION_CONTEXT_PREFIX <= s)
-  {
-    assert && ENCRYPTION_CONTEXT_PREFIX[0] == 'a'
-           && HIERARCHY_VERSION[0] == 'h'
-           && 'a' != 'h';
-  }
-
-  lemma RestrictedStringsEnsureNotPrefixed(s: string)
-    requires s in BRANCH_KEY_RESTRICTED_FIELD_NAMES
-    ensures !(ENCRYPTION_CONTEXT_PREFIX <= s)
-  {
-    assert && ENCRYPTION_CONTEXT_PREFIX[0] == 'a'
-           && HIERARCHY_VERSION[0] == 'h'
-           && 'a' != 'h';
-  }
-
-  lemma PrefixedStringsAreNotReserved(s: string)
-    requires ENCRYPTION_CONTEXT_PREFIX <= s
-    ensures s !in BRANCH_KEY_RESTRICTED_FIELD_NAMES
-  {
-    assert && ENCRYPTION_CONTEXT_PREFIX[0] == 'a'
-           && HIERARCHY_VERSION[0] == 'h'
-           && 'a' != 'h';
-  }
+  lemma HierarchyVersionIsNotPrefixed()
+    ensures ENCRYPTION_CONTEXT_PREFIX[0] == 'a'
+            && HIERARCHY_VERSION[0] == 'h'
+            && "a" != "h"
+  {}
 
   type PrefixedEncryptionContext = m: map<string, string> | PrefixedEncryptionContext?(m) witness *
   predicate PrefixedEncryptionContext?(m: map<string, string>): (output: bool)
@@ -488,7 +467,7 @@ module {:options "/functionSyntax:4" } Structure {
     Success(map i <- encodedEncryptionContext :: i.0.value := i.1.value)
   }
 
-  opaque function DecryptOnlyBranchKeyEncryptionContext(
+  function DecryptOnlyBranchKeyEncryptionContext(
     branchKeyId: string,
     branchKeyVersion: string,
     timestamp: string,
@@ -499,6 +478,7 @@ module {:options "/functionSyntax:4" } Structure {
   ): (output: map<string, string>)
     requires 0 < |branchKeyId|
     requires 0 < |branchKeyVersion|
+    // TODO: Rustan suggests replacing all of these post-conditions with the lambda
     ensures BranchKeyContext?(output)
     ensures BRANCH_KEY_TYPE_PREFIX < output[TYPE_FIELD]
     ensures BRANCH_KEY_ACTIVE_VERSION_FIELD !in output
@@ -511,56 +491,61 @@ module {:options "/functionSyntax:4" } Structure {
                 && output[ENCRYPTION_CONTEXT_PREFIX + k] == encryptionContext[k]
     ensures PrefixedEncryptionContext?(output - BRANCH_KEY_RESTRICTED_FIELD_NAMES)
   {
-    // Dafny needs some help.
-    // Adding a fixed string
-    // will not make any of the keys collide.
-    // However, this leaks a lot of complexity.
-    // This is why the function is now opaque.
-    // Otherwise things timeout
-    assert forall k <- encryptionContext.Keys
-        ::
-          && k == (ENCRYPTION_CONTEXT_PREFIX + k)[|ENCRYPTION_CONTEXT_PREFIX|..];
-    // TODO-HV-2-FOLLOW : Using a Match statement to set the HIERARCHY_VERSION has made Dafny
-    // doubt that the prefixed-EC is disjoint from the reserved words.
-    // While this is really interesting, we KNOW this is true, and I am not going to spend.
-    // I would like to make some tiny functions that handle just prefixing...
     var prefixedEncryptionContext :=
-      map k <- encryptionContext :: ENCRYPTION_CONTEXT_PREFIX + k := encryptionContext[k];
-    // assume {:axiom} forall k :: k in prefixedEncryptionContext.Keys ==> ENCRYPTION_CONTEXT_PREFIX <= k;
-    // assume {:axiom} prefixedEncryptionContext.Keys !! BRANCH_KEY_RESTRICTED_FIELD_NAMES;
-    assert
-      (
-        (forall k :: k in prefixedEncryptionContext.Keys
-                     ==>
-                       ENCRYPTION_CONTEXT_PREFIX <= k)
-        &&
-        (
-          forall
-            reserved <- BRANCH_KEY_RESTRICTED_FIELD_NAMES
-            ::
-              !( ENCRYPTION_CONTEXT_PREFIX <= reserved) && !(ENCRYPTION_CONTEXT_PREFIX < reserved)
-        )
-        ==> PrefixedEncryptionContext?(prefixedEncryptionContext)
+      PrefixUtils.AddingPrefixToKeysOfMapDoesNotCreateCollisions(
+        prefix := ENCRYPTION_CONTEXT_PREFIX,
+        aMap := encryptionContext
       );
-    assert forall k <- encryptionContext.Keys
-        ::
-          && ENCRYPTION_CONTEXT_PREFIX + k in prefixedEncryptionContext
-          && prefixedEncryptionContext[ENCRYPTION_CONTEXT_PREFIX + k] == encryptionContext[k];
+    var requiredFields :=
+      map[
+        BRANCH_KEY_IDENTIFIER_FIELD := branchKeyId,
+        TYPE_FIELD := BRANCH_KEY_TYPE_PREFIX + branchKeyVersion,
+        KEY_CREATE_TIME := timestamp,
+        TABLE_FIELD := logicalKeyStoreName,
+        KMS_FIELD := kmsKeyArn,
+        HIERARCHY_VERSION := HierarchyVersionToString(hierarchyVersion)
+      ];
+    assert (forall k <- requiredFields.Keys :: k !in prefixedEncryptionContext)
+    by {
+      NoRestrictedAttributeNameStartsWithPrefix();
 
-    var output := prefixedEncryptionContext + map[
-                    BRANCH_KEY_IDENTIFIER_FIELD := branchKeyId,
-                    TYPE_FIELD := BRANCH_KEY_TYPE_PREFIX + branchKeyVersion,
-                    KEY_CREATE_TIME := timestamp,
-                    TABLE_FIELD := logicalKeyStoreName,
-                    KMS_FIELD := kmsKeyArn,
-                    HIERARCHY_VERSION := HierarchyVersionToString(hierarchyVersion)
-                  ];
-    assert forall k <- encryptionContext.Keys
-        ::
-          && ENCRYPTION_CONTEXT_PREFIX + k in prefixedEncryptionContext
-          && output[ENCRYPTION_CONTEXT_PREFIX + k] == encryptionContext[k];
+    }
+    var output := prefixedEncryptionContext + requiredFields;
     output
   }
+
+  lemma AboutDecryptOnlyBranchKeyContext(
+    branchKeyId: string,
+    branchKeyVersion: string,
+    timestamp: string,
+    logicalKeyStoreName: string,
+    kmsKeyArn: string,
+    hierarchyVersion: Types.HierarchyVersion,
+    encryptionContext: map<string, string>
+  )
+    requires 0 < |branchKeyId|
+    requires 0 < |branchKeyVersion|
+    ensures var output := DecryptOnlyBranchKeyEncryptionContext(
+                            branchKeyId, branchKeyVersion, timestamp, logicalKeyStoreName,
+                            kmsKeyArn, hierarchyVersion, encryptionContext
+                          );
+            && BranchKeyContext?(output)
+  {
+    var output := DecryptOnlyBranchKeyEncryptionContext(
+      branchKeyId, branchKeyVersion, timestamp, logicalKeyStoreName,
+      kmsKeyArn, hierarchyVersion, encryptionContext
+    );
+    assert BRANCH_KEY_TYPE_PREFIX < output[TYPE_FIELD];
+    assert BRANCH_KEY_ACTIVE_VERSION_FIELD !in output;
+    assert output[KMS_FIELD] == kmsKeyArn;
+    assert output[TABLE_FIELD] == logicalKeyStoreName;
+    assert output[HIERARCHY_VERSION] == HierarchyVersionToString(hierarchyVersion);
+    assert forall k <- encryptionContext.Keys :: ENCRYPTION_CONTEXT_PREFIX + k in output;
+    assert forall k <- encryptionContext.Keys :: output[ENCRYPTION_CONTEXT_PREFIX + k] == encryptionContext[k];
+    assert PrefixedEncryptionContext?(output - BRANCH_KEY_RESTRICTED_FIELD_NAMES);
+    assert BranchKeyContext?(output);
+  }
+
 
   function ActiveBranchKeyEncryptionContext(
     decryptOnlyEncryptionContext: map<string, string>
